coq/clc_semantics_bak0/clc_ast.v
@@ -10,7 +10,7 @@ Inductive term : Type :=
 | Var    (x : var)
 | Sort   (s : sort) (l : nat)
 | Pi     (A : term) (B : {bind term}) (s r t : sort)
-| Lam    (A : term) (m : {bind term}) (s t : sort)
+| Lam    (m : {bind term}) (s t : sort)
 | App    (m n : term)
 | Unit
 | It
@@ -29,14 +29,11 @@ Instance substLemmas_term : SubstLemmas term. derive. Qed.
 
 Reserved Notation "m ~> n" (at level 30).
 Inductive step : term -> term -> Prop :=
-| step_beta A m n s t :
-  (App (Lam A m s t) n) ~> m.[n/]
-| step_lamL A A' m s t :
-  A ~> A' ->
-  Lam A m s t ~> Lam A' m s t
-| step_lamR A m m' s t :
+| step_beta m n s t :
+  (App (Lam m s t) n) ~> m.[n/]
+| step_lam m m' s t :
   m ~> m' ->
-  Lam A m s t ~> Lam A m' s t
+  Lam m s t ~> Lam m' s t
 | step_piL A A' B s r t :
   A ~> A' ->
   Pi A B s r t ~> Pi A' B s r t
